Semantics/IRTreeEval.thy
@@ -418,4 +418,23 @@ lemma not_down_up_mask_and_zero_implies_zero:
 
 end
 
+definition IRExpr_up :: "IRExpr \<Rightarrow> int64" where
+  "IRExpr_up e = not 0"
+
+definition IRExpr_down :: "IRExpr \<Rightarrow> int64" where
+  "IRExpr_down e = 0"
+
+lemma ucast_zero: "(ucast (0::int64)::int32) = 0"
+  by simp
+
+lemma ucast_minus_one: "(ucast (-1::int64)::int32) = -1"
+  apply transfer by auto
+
+interpretation simple_mask: stamp_mask
+  "IRExpr_up :: IRExpr \<Rightarrow> int64"
+  "IRExpr_down :: IRExpr \<Rightarrow> int64"
+  unfolding IRExpr_up_def IRExpr_down_def
+  apply unfold_locales
+  by (simp add: ucast_minus_one)+
+
 end
